full proof of bv_extract using words...

src/bva/Bva_checker.v
@@ -764,7 +764,84 @@ Fixpoint check_symopp (bs1 bs2 bsres : list _lit) (bvop: binop)  :=
       end
     else C._true.
 
- 
+
+
+  (** Checker for bitvector extraction *)
+  Fixpoint extract_lit (x: list _lit) (i j: nat) : list _lit :=
+    match x with
+      | []         => []
+      | bx :: x'   => 
+        match i with
+          | O      =>
+            match j with
+              | O    => []
+              | S j' => bx :: extract_lit x' i j'
+            end
+          | S i'   => 
+            match j with
+              | O    => []
+              | S j' => extract_lit x' i' j'
+            end
+        end
+   end.
+
+   Definition check_extract (bs bsres: list _lit) (i j: nat) : bool :=
+     if (Nat.ltb (length bs) j) 
+     then false
+     else
+       if (forallb2 eq_carry_lit (lit_to_carry (extract_lit bs i j)) bsres)
+       then true
+       else false.
+
+  Definition check_extract3 (bs bsres: list _lit) (i j: N) : bool :=
+    forallb2 (fun l1 l2 => l1 == l2) (extract_lit bs (nat_of_N i) (nat_of_N j)) bsres.
+
+
+  (** Checker for bitvector extraction *)
+  Fixpoint check_extract2 (x bsres: list _lit) (i j: nat) : bool :=
+    match x with
+      | [] => match bsres with [] => true | _ => false end
+      | bx :: x' => 
+        match i with
+          | O      =>
+            match j, bsres with
+            | O, nil => true
+            | S j', b :: bsres' => (bx == b) && check_extract2 x' bsres' i j'
+            | _, _ => false
+            end
+          | S i'   => 
+            match j, bsres with
+              | O, nil => true
+              | S j', _ => check_extract2 x' bsres i' j'
+              | _, _ => false
+            end
+        end
+   end.
+
+  Definition check_bbExtract s pos lres :=
+    match S.get s pos with
+      | l1::nil =>
+        if (Lit.is_pos l1) && (Lit.is_pos lres) then
+          match get_form (Lit.blit l1), get_form (Lit.blit lres) with
+            | FbbT a1 bs, FbbT a bsres =>
+              match get_atom a with
+
+                | Auop (UO_BVextr i n0 n1) a1' =>
+                  if ((a1 == a1') (* || ((a1 == a2') && (a2 == a1')) *) )
+                       && (check_extract bs bsres i (n0 + i))
+                       && ((length bs) =? n1)%nat
+                       && (Nat.leb (n0 + i) n1)
+                  then lres::nil
+                  else C._true
+
+                | _ => C._true
+              end
+            | _, _ => C._true
+          end
+        else C._true
+      | _ => C._true
+    end.
+
 (*
 
   Variable s : S.t.
@@ -819,82 +896,6 @@ Fixpoint check_symopp (bs1 bs2 bsres : list _lit) (bvop: binop)  :=
 
 
 
-
-  (** Checker for bitvector extraction *)
-  Fixpoint extract_lit (x: list _lit) (i j: nat) : list _lit :=
-    match x with
-      | []         => []
-      | bx :: x'   => 
-        match i with
-          | O      =>
-            match j with
-              | O    => []
-              | S j' => bx :: extract_lit x' i j'
-            end
-          | S i'   => 
-            match j with
-              | O    => []
-              | S j' => extract_lit x' i' j'
-            end
-        end
-   end.
-
-   Definition check_extract (bs bsres: list _lit) (i j: N) : bool :=
-     if (N.ltb (N.of_nat (length bs)) j) 
-     then false
-     else
-       if (forallb2 eq_carry_lit (lit_to_carry (extract_lit bs (nat_of_N i) (nat_of_N j))) bsres)
-       then true
-       else false.
-
-  Definition check_extract3 (bs bsres: list _lit) (i j: N) : bool :=
-    forallb2 (fun l1 l2 => l1 == l2) (extract_lit bs (nat_of_N i) (nat_of_N j)) bsres.
-
-
-  (** Checker for bitvector extraction *)
-  Fixpoint check_extract2 (x bsres: list _lit) (i j: nat) : bool :=
-    match x with
-      | [] => match bsres with [] => true | _ => false end
-      | bx :: x' => 
-        match i with
-          | O      =>
-            match j, bsres with
-            | O, nil => true
-            | S j', b :: bsres' => (bx == b) && check_extract2 x' bsres' i j'
-            | _, _ => false
-            end
-          | S i'   => 
-            match j, bsres with
-              | O, nil => true
-              | S j', _ => check_extract2 x' bsres i' j'
-              | _, _ => false
-            end
-        end
-   end.
-
-  Definition check_bbExtract s pos lres :=
-    match S.get s pos with
-      | l1::nil =>
-        if (Lit.is_pos l1) && (Lit.is_pos lres) then
-          match get_form (Lit.blit l1), get_form (Lit.blit lres) with
-            | FbbT a1 bs, FbbT a bsres =>
-              match get_atom a with
-
-                | Auop (UO_BVextr i n0 n1) a1' =>
-                  if ((a1 == a1') (* || ((a1 == a2') && (a2 == a1')) *) )
-                       && (check_extract bs bsres i (n0 + i))
-                       && (N.of_nat (length bs) =? n1)%N
-                       && (N.leb (n0 + i) n1)
-                  then lres::nil
-                  else C._true
-
-                | _ => C._true
-              end
-            | _, _ => C._true
-          end
-        else C._true
-      | _ => C._true
-    end.
 
 *)
 
@@ -1214,6 +1215,7 @@ Proof. intros a bs.
          omega.
          intro H3. rewrite H3 in H0. now contradict H0.
          intros i3 n0 n1 Heq. rewrite Heq in H0. now contradict H0.
+         intros b0 i2 i3 Heq. rewrite Heq in H0. now contradict H0.
          intros n0 i2 i3 i4 Heq. rewrite Heq in H0. now contradict H0.
          intros n0 i3 Heq. rewrite Heq in H0. now contradict H0. 
          intros  i2 i3 Heq. rewrite Heq in H0. now contradict H0.
@@ -3142,7 +3144,7 @@ Proof.
       case_eq (t_form .[ Lit.blit lres]); try (intros; now apply C.interp_true).
       intros a bsres Heq5.
       case_eq (t_atom .[ a]); try (intros; now apply C.interp_true).
-      intros [ | | | | | | | | | ]  a1'  Heq6; try (intros; now apply C.interp_true).
+      intros [ | | | | | | | | | | ]  a1'  Heq6; try (intros; now apply C.interp_true).
       (* BVzextend *)
     - case_eq ((a1 == a1')); simpl; intros Heq7; try (now apply C.interp_true).
         case_eq (
@@ -3264,6 +3266,382 @@ Proof.
         rewrite map_length in H101. rewrite <- H101.
         now apply zextend_interp_main.
 Qed.
+
+
+Lemma extract_interp_zero: forall a n, RAWBITVECTOR_LIST.extract (map (Lit.interp rho) a) 0 n =
+map (Lit.interp rho) (extract_lit a 0 n).
+Proof. intro a.
+       induction a as [ | xa xsa IHa].
+       - intros. now simpl.
+       - intros. simpl.
+         case_eq n.
+         now simpl.
+         intros. simpl. apply f_equal.
+         now rewrite IHa.
+Qed.
+
+Lemma extract_interp_all: forall a m n, RAWBITVECTOR_LIST.extract (map (Lit.interp rho) a) m n =
+map (Lit.interp rho) (extract_lit a m n).
+Proof. intro a.
+       induction a as [ | xa xsa IHa].
+       - intros. now simpl.
+       - intros. case_eq m.
+         intros. apply extract_interp_zero.
+         intros. simpl.         
+         case_eq n.
+         now simpl.
+         intros. simpl.
+         now rewrite IHa.
+Qed.
+
+Lemma N_minus_n_O: forall n, (n - 0)%N = n.
+Proof. intros. lia. Qed.
+
+Lemma len_extr: forall n a, 
+(Datatypes.length a) >= n ->
+(Datatypes.length (RAWBITVECTOR_LIST.extract a 0 n)) = n.
+Proof. intros. case_eq n; intros.
+       case_eq a; intros; now simpl.
+       specialize (@RAWBITVECTOR_LIST.length_extract a (N.of_nat 0) (N.of_nat n)); intros.
+       rewrite !Nat2N.id in H1. simpl in H1. rewrite <- H0.
+       
+       rewrite N_minus_n_O in H1.
+       rewrite !Nat2N.id in H1.
+       rewrite H1. easy. lia. rewrite H0. lia.
+Qed.
+
+Lemma len_extr_lit: forall a n,
+(Datatypes.length a) >= n ->
+(Datatypes.length (map (Lit.interp rho) (extract_lit a 0 n))) = n.
+Proof. intros. 
+       rewrite <- extract_interp_all, len_extr. easy.
+       rewrite map_length. easy.
+Qed.
+
+Lemma extract_interp_main: forall bs1 bsres (i n0: nat),
+                  check_extract bs1 bsres i (n0 + i) = true ->
+                  wextr (ListToword (map (Lit.interp rho) bs1) (length bs1)) i (i + n0) n0 
+                  = ListToword (map (Lit.interp rho) bsres) n0.
+Proof. intro bs1.
+       induction bs1 as [ | xbs1 xsbs1 IHbs1].
+       - intros. simpl. unfold wextr. simpl.
+         unfold check_extract in H. simpl in H.
+         case_eq ((0 <? n0 + i)); intros.
+         rewrite H0 in H. now contradict H.
+         rewrite H0 in H.
+         case_eq bsres; intros. now simpl.
+          intros. rewrite H1 in H. now contradict H.
+       - intros. unfold check_extract in H.
+         case_eq (((Datatypes.length (xbs1 :: xsbs1)) <? n0 + i)); intros.
+         rewrite H0 in H. now contradict H.
+         rewrite H0 in H.
+         case_eq (
+          forallb2 eq_carry_lit
+          (lit_to_carry
+          (extract_lit (xbs1 :: xsbs1) 
+          i ((n0 + i)))) bsres); intros.
+         apply prop_eq_carry_lit2 in H1.
+         rewrite prop_interp_carry3 in H1.
+         simpl in H1. simpl.
+
+         unfold wextr. rewrite W2L_involutive.
+         case_eq i; intros; rewrite H2 in H1.
+         case_eq (n0)%nat; intros; rewrite H3 in H1.
+         simpl in H1.  rewrite <- H1. now simpl.
+         simpl in H1. simpl. rewrite plus_0_r in H1.
+         specialize (helper_strong (RAWBITVECTOR_LIST.extract (map (Lit.interp rho) xsbs1) 0 n)
+                                   (Lit.interp rho xbs1 )); intros.
+         rewrite len_extr in H4.
+         rewrite H4, <- H1. simpl.
+         specialize (helper_strong (map (Lit.interp rho) (extract_lit xsbs1 0 n))
+                                   (Lit.interp rho xbs1 )); intros.
+         rewrite len_extr_lit in H5.
+         rewrite H5. apply f_equal. now rewrite extract_interp_all.
+         rewrite <- H2 in H1. simpl in H0. rewrite H2, H3 in H0.
+         apply Nat.ltb_ge in H0. lia. rewrite map_length.
+         rewrite <- H2 in H1. simpl in H0. rewrite H2, H3 in H0.
+         apply Nat.ltb_ge in H0. lia. 
+
+         rewrite <- H2 in H1.
+         case_eq ((n0 + i)%nat); intros; rewrite H3 in H1.
+         rewrite <- H2. rewrite Nat.add_comm in H3. rewrite H3.
+         rewrite <- H1. simpl. case_eq i; easy.
+         rewrite <- H2. rewrite Nat.add_comm in H3. rewrite H3.
+         simpl. rewrite H2. now rewrite extract_interp_all, H1.
+         simpl. now rewrite map_length.
+         
+         rewrite H1 in H. now contradict H.
+Qed.
+
+Lemma inj_ge: forall a b c, (N.of_nat a >= N.of_nat (b + c))%N <-> a >= (b + c).
+Proof. intros. lia. Qed.
+
+Lemma res_len: forall a b (i n: nat), check_extract a b i (n + i) = true -> length b = n.
+Proof. intro a.
+       induction a as [ | xa xsa IHa ]; intros.
+       - simpl in H. unfold check_extract in H.
+         simpl in H. case_eq (0 <? n + i); intros; rewrite H0 in H.
+         now contradict H0.
+         case_eq b; intros; rewrite H1 in H.
+         case_eq n; intros. now simpl. subst. now contradict H0.
+         now contradict H.
+       - simpl in H. unfold check_extract in H.
+         case_eq (Datatypes.length (xa :: xsa) <? n + i); intros; rewrite H0 in H.
+         now contradict H.
+         case_eq (forallb2 eq_carry_lit (lit_to_carry (extract_lit (xa :: xsa) i (n + i))) b); intros;
+         rewrite H1 in H.
+         apply prop_eq_carry_lit2 in H1.
+         rewrite prop_interp_carry3 in H1.
+         rewrite <- extract_interp_all in H1.
+         assert ( length (RAWBITVECTOR_LIST.extract (map (Lit.interp rho) (xa :: xsa)) i (n + i)) =
+                  length (map (Lit.interp rho) b)). { now rewrite H1. }
+         specialize (@RAWBITVECTOR_LIST.length_extract (map (Lit.interp rho) (xa :: xsa)) (N.of_nat i) (N.of_nat (n + i))); intros.
+         rewrite Nat2N.id in H3. assert ((N.to_nat (N.of_nat (n + i))) = (n + i)%nat). { lia. }
+         assert (N.to_nat (N.of_nat (n + i) - N.of_nat i) = n). { lia. }
+         rewrite H4, H5 in H3. rewrite H3 in H2. now rewrite map_length in H2.
+         rewrite map_length. apply Nat.ltb_ge in H0. apply inj_ge. lia. lia.
+         now contradict H.
+Qed.
+
+  Lemma Npos_dist: forall p p0: positive, (Npos (p + p0))%N = (Npos p + Npos p0)%N.
+  Proof. intros. case p in *; case p0 in *; easy. Qed.
+
+  Lemma not_ltb2: forall (n0 n1 i: N), (n1 >= n0 + i)%N -> (n1 <? n0 + i)%N = false.
+  Proof. intro n0.
+         induction n0.
+         intros. simpl in *.
+         now apply N.ltb_nlt in H.
+
+         intros. simpl.
+         case_eq i.
+         intros. subst. simpl in H.
+         now apply N.ltb_nlt in H.
+         intros. subst.
+         apply N.ltb_nlt in H.
+         now rewrite Npos_dist.
+  Qed.
+
+  Lemma not_ltb3: forall (n0 n1 i: nat), (n1 >= n0 + i)%nat -> (n1 <? n0 + i)%nat = false.
+  Proof. intro n0.
+         induction n0.
+         intros. simpl in *.
+         now apply Nat.ltb_ge in H.
+
+         intros. simpl.
+         case_eq i.
+         intros. subst. simpl in H.
+         now apply Nat.ltb_ge in H.
+         intros. subst.
+         now apply Nat.ltb_ge in H.
+  Qed.
+
+Lemma l2w_eq: forall a b n,
+(length a = n) -> (length b = n) ->
+ListToword a n = ListToword b n -> a = b.
+Proof. intro a.
+       induction a as [ | xa xsa IHa ]; intros.
+       - simpl in H. symmetry in H. rewrite H in H0. now rewrite empty_list_length in H0.
+       - simpl in *. case_eq b; intros. subst. now contradict H0.
+         rewrite <- H in H1.
+         rewrite helper_strong in H1. rewrite H2 in H0.
+         rewrite <- H in H0. inversion H0. rewrite <- H4 in H1. rewrite H2 in H1.
+         rewrite helper_strong in H1. inversion H1. rewrite H5 in H1.
+         apply f_equal. apply IHa with (n - 1)%nat. lia. rewrite <- H.
+         lia. assert ((n - 1)%nat = (length l)). { lia. }
+         
+         rewrite H3. 
+         now dependent rewrite -> H6.
+Qed.
+
+Lemma valid_check_bbExtract s pos lres : C.valid rho (check_bbExtract s pos lres).
+Proof.
+      unfold check_bbExtract.
+      case_eq (S.get s pos); [intros _|intros l1 [ |l] Heq1]; try now apply C.interp_true.
+      case_eq (Lit.is_pos l1); intro Heq2; simpl; try now apply C.interp_true.
+      case_eq (Lit.is_pos lres); intro Heq3; simpl; try now apply C.interp_true.
+      case_eq (t_form .[ Lit.blit l1]); try (intros; now apply C.interp_true). intros a1 bs1 Heq4.
+      case_eq (t_form .[ Lit.blit lres]); try (intros; now apply C.interp_true).
+      intros a bsres Heq5.
+      case_eq (t_atom .[ a]); try (intros; now apply C.interp_true).
+      intros [ | | | | | | | | | | ]  a1'  Heq6; try (intros; now apply C.interp_true).
+      (* BVextract *)
+    - case_eq ((a1 == a1')); simpl; intros Heq7; try (now apply C.interp_true).
+        case_eq (
+          check_extract bs1 bsres i (n0 + i) &&
+          ( (Datatypes.length bs1) =? n1)%nat && (n0 + i <=? n1)%nat
+        ); simpl; intros Heq8; try (now apply C.interp_true).
+
+        unfold C.valid. simpl. rewrite orb_false_r.
+        unfold Lit.interp. rewrite Heq3.
+        unfold Var.interp.
+        rewrite wf_interp_form; trivial. rewrite Heq5. simpl.
+
+        apply weqb_true_iff.
+
+        generalize wt_t_atom. unfold Atom.wt. unfold is_true.
+        rewrite PArray.forallbi_spec;intros.
+
+        pose proof (H a). 
+        assert (a < PArray.length t_atom).
+        { apply PArray.get_not_default_lt. rewrite def_t_atom. rewrite Heq6. easy. }
+        specialize (@H0 H1). rewrite Heq6 in H0. simpl in H0.
+        rewrite !andb_true_iff in H0. destruct H0.
+
+        unfold get_type' in H0. unfold v_type in H0.
+        case_eq (t_interp .[ a]).
+        intros v_typea v_vala Htia. rewrite Htia in H0.
+        case_eq (v_typea);  intros; rewrite H3 in H0; try (now contradict H2).
+        rename H0 into Hv.
+
+        generalize (Hs s pos). intros HSp. unfold C.valid in HSp. rewrite Heq1 in HSp.
+        unfold C.interp in HSp. unfold existsb in HSp. rewrite orb_false_r in HSp.
+        unfold Lit.interp in HSp. rewrite Heq2 in HSp. unfold Var.interp in HSp.
+        rewrite rho_interp in HSp. rewrite Heq4 in HSp. simpl in HSp.
+
+        apply weqb_true_iff in HSp.
+
+        unfold get_type' in H2. unfold v_type in H2.
+        case_eq (t_interp .[ a1']).
+          intros v_typea1 v_vala1 Htia1. rewrite Htia1 in H2.
+        rewrite Atom.t_interp_wf in Htia1; trivial.
+        unfold apply_binop.
+        apply Typ.eqb_spec in H2.
+
+        (** case a1 = a1' **)
+        rewrite eqb_spec in Heq7; rewrite Heq7 in *.
+
+        (* interp_form_hatom_bv a = 
+                interp_bv t_i (interp_atom (t_atom .[a])) *)
+        assert (interp_form_hatom_word a = 
+                interp_word t_i (interp_atom (t_atom .[a]))).
+        {
+          rewrite !Atom.t_interp_wf in Htia; trivial.
+          rewrite Htia.
+          unfold Atom.interp_form_hatom_word.
+          unfold Atom.interp_hatom.
+          rewrite !Atom.t_interp_wf; trivial.
+          rewrite Htia. easy.
+        }
+
+        rewrite H0. rewrite Heq6. simpl.
+        unfold interp_word. unfold apply_unop.
+
+        rewrite !Atom.t_interp_wf; trivial.
+
+        revert v_vala1 Htia1. rewrite H2.
+        intros v_vala1 Htia1.
+        rewrite Htia1.
+        rewrite !Typ.cast_refl.
+        unfold Bval.
+
+        assert (H100: ((Datatypes.length (map (Lit.interp rho) bsres))) = n0).
+        { rewrite map_length. specialize (@res_len bs1 bsres i n0); intros.
+          apply H4.
+           rewrite !andb_true_iff in Heq8.
+           now destruct Heq8 as ((Heq8a, Heq8b), Heq8c).
+        }
+
+        rewrite H100.
+        rewrite Typ.cast_refl. intros.
+        simpl.
+
+        (* interp_form_hatom_bv a1' = 
+                interp_bv t_i (interp_atom (t_atom .[a1'])) *)
+        assert (interp_form_hatom_word a1' = 
+                interp_word t_i (interp_atom (t_atom .[a1']))).
+        {
+          rewrite !Atom.t_interp_wf in Htia; trivial.
+          rewrite Htia1.
+          unfold Atom.interp_form_hatom_word.
+          unfold Atom.interp_hatom.
+          rewrite !Atom.t_interp_wf; trivial.
+          rewrite Htia1. easy.
+        }
+
+        rewrite H4 in HSp.
+        unfold interp_word in HSp.
+        rewrite Htia1 in HSp.
+        unfold interp_word in HSp. 
+
+        revert HSp.
+
+        assert (H101: ((Datatypes.length (map (Lit.interp rho) bs1))) = n1).
+        {  rewrite !andb_true_iff in Heq8.
+           destruct Heq8 as ((Heq8a, Heq8b), Heq8c).
+           rewrite map_length.
+           now rewrite Nat.eqb_eq in Heq8b.
+        }
+
+
+        rewrite H101.
+        rewrite Typ.cast_refl. intros.
+        simpl.
+
+        rewrite HSp. simpl.
+        unfold wextr.
+        rewrite !andb_true_iff in Heq8.
+        destruct Heq8 as (Heq8a, Heq8b).
+        specialize (@extract_interp_main bs1 bsres i n0).
+        intros.
+        rewrite map_length in H101.
+        rewrite H101 in H5. unfold wextr in H5. now rewrite H5.
+Qed.
+
+
+(*
+
+Lemma sextend_interp_zero: forall a, RAWBITVECTOR_LIST.sextend (map (Lit.interp rho) a) O =
+(map (Lit.interp rho) (sextend_lit a 0)).
+Proof. intros.
+       unfold RAWBITVECTOR_LIST.sextend.
+       case_eq a; intros; now simpl.
+Qed.
+
+Lemma sextend_interp_empty: forall i, RAWBITVECTOR_LIST.sextend (map (Lit.interp rho) []) i =
+map (Lit.interp rho) (sextend_lit [] i).
+Proof. simpl. intro i.
+       induction i.
+       - intros. now simpl.
+       - intros. simpl.
+         unfold RAWBITVECTOR_LIST.sextend in *.
+         simpl. rewrite IHi.
+         assert (Lit.interp rho Lit._false = false).
+           { specialize (Lit.interp_false rho wf_rho). intros.
+              rewrite <- not_true_iff_false.
+              unfold not in *.
+              intros. now apply H. }
+        now rewrite H.
+ Qed.
+
+Lemma sextend_interp_all: forall a i, RAWBITVECTOR_LIST.sextend (map (Lit.interp rho) a) i =
+map (Lit.interp rho) (sextend_lit a i).
+Proof. intro a.
+       induction a as [ | xa xsa IHa].
+       - intros. simpl.
+         induction i.
+         + intros. now simpl.
+         + intros. unfold RAWBITVECTOR_LIST.sextend in *.
+           simpl. rewrite IHi.
+           assert (Lit.interp rho Lit._false = false).
+           { specialize (Lit.interp_false rho wf_rho). intros.
+              rewrite <- not_true_iff_false.
+              unfold not in *.
+              intros. now apply H. }
+           now rewrite H.
+        - intros. 
+          induction i.
+          + now simpl.
+          + unfold RAWBITVECTOR_LIST.sextend, zextend_lit in *.
+            simpl in *. rewrite <- IHi.
+           assert (Lit.interp rho Lit._false = false).
+           { specialize (Lit.interp_false rho wf_rho). intros.
+              rewrite <- not_true_iff_false.
+              unfold not in *.
+              intros. now apply H. }
+           reflexivity.
+Qed.
+
+*)
 
 (** BV ADDITION CHECKER WORDS*)
 
@@ -6671,7 +7049,7 @@ Proof.
       case_eq (t_form .[ Lit.blit lres]); try (intros; now apply C.interp_true).
       intros a bsres Heq8.
       case_eq (t_atom .[ a]); try (intros; now apply C.interp_true).
-      intros [ | | | | | | | | | ] a1' Heq9; try now apply C.interp_true.
+      intros [ | | | | | | | | | | ] a1' Heq9; try now apply C.interp_true.
 
       case_eq ((a1 == a1') && check_neg bs1 bsres &&
       ((Datatypes.length bs1) =? n)%nat); 
@@ -7643,7 +8021,21 @@ Proof.
 Qed.
 
 
+
 (** incorporated down here *)
+
+
+(*
+Lemma prop_check_slt: forall a b, 
+  length a = length b ->
+    Word.wsltbZ (ListToword a (length a)) (ListToword b (length a))
+    = 
+    RAWBITVECTOR_LIST.slt_list a b. 
+Proof. intros. rewrite <- wsltZ_true_iff. rewrite W2L_involutive.
+       rewrite H, W2L_involutive. reflexivity. easy. easy.
+Qed.
+
+*)
 
 
 (*
@@ -10412,347 +10804,6 @@ Proof.
 Qed.
 
 
-
-Lemma extract_interp_zero: forall a n, RAWBITVECTOR_LIST.extract (map (Lit.interp rho) a) 0 n =
-map (Lit.interp rho) (extract_lit a 0 n).
-Proof. intro a.
-       induction a as [ | xa xsa IHa].
-       - intros. now simpl.
-       - intros. simpl.
-         case_eq n.
-         now simpl.
-         intros. simpl. apply f_equal.
-         now rewrite IHa.
-Qed.
-
-Lemma extract_interp_all: forall a m n, RAWBITVECTOR_LIST.extract (map (Lit.interp rho) a) m n =
-map (Lit.interp rho) (extract_lit a m n).
-Proof. intro a.
-       induction a as [ | xa xsa IHa].
-       - intros. now simpl.
-       - intros. case_eq m.
-         intros. apply extract_interp_zero.
-         intros. simpl.         
-         case_eq n.
-         now simpl.
-         intros. simpl.
-         now rewrite IHa.
-Qed.
-
-Lemma extract_interp_main: forall bs1 bsres (i n0: N),
-                  check_extract bs1 bsres i (n0 + i) = true ->
-                  @RAWBITVECTOR_LIST.bv_extr i n0 (N.of_nat (length bs1)) 
-                    (map (Lit.interp rho) bs1) = map (Lit.interp rho) bsres.
-Proof. intro bs1.
-       induction bs1 as [ | xbs1 xsbs1 IHbs1].
-       - intros. simpl.
-         unfold check_extract in H. simpl in H.
-         unfold RAWBITVECTOR_LIST.bv_extr.
-          case_eq (nat_of_N i).
-          intros. simpl.
-          case_eq (nat_of_N n0).
-          intros. simpl.
-         case_eq ((0 <? n0 + i)%N); intros.
-          rewrite H2 in H. now contradict H.
-          rewrite H2 in H.
-         case_eq bsres. intros. now simpl.
-          intros. rewrite H3 in H. now contradict H.
-          intros.
-          case_eq bsres. intros.
-          apply (f_equal (N.of_nat)) in H1.
-          apply (f_equal (N.of_nat)) in H0.
-          rewrite N2Nat.id in H1, H0. rewrite H1, H0 in H.
-          simpl in H. now contradict H0.
-          intros. rewrite H2 in H.
-          case ((0 <? n0 + i)%N) in H; now contradict H.
-          intros.
-          case_eq (N.to_nat n0).
-          intros.
-          apply (f_equal (N.of_nat)) in H1.
-          apply (f_equal (N.of_nat)) in H0.
-          rewrite N2Nat.id in H1, H0. rewrite H1, H0 in H.
-          simpl in H. now contradict H0.
-          intros.
-          apply (f_equal (N.of_nat)) in H1.
-          apply (f_equal (N.of_nat)) in H0.
-          rewrite N2Nat.id in H1, H0. rewrite H1, H0 in H.
-          simpl in H. now contradict H0.
-       - intros. unfold check_extract in H.
-         case_eq ((N.of_nat (Datatypes.length (xbs1 :: xsbs1)) <? n0 + i)%N).
-         intros. rewrite H0 in H. now contradict H.
-         intros. rewrite H0 in H.         
-         case_eq (
-          forallb2 eq_carry_lit
-          (lit_to_carry
-          (extract_lit (xbs1 :: xsbs1) 
-          (N.to_nat i) (N.to_nat (n0 + i)))) bsres); intros.
-         apply prop_eq_carry_lit2 in H1.
-         rewrite prop_interp_carry3 in H1.
-         simpl in H1. simpl.
-
-         unfold RAWBITVECTOR_LIST.bv_extr in *.
-         simpl in *.
-         case_eq (N.to_nat i); intros; rewrite H2 in H1.
-         case_eq (N.to_nat (n0 + i)); intros; rewrite H3 in H1.
-         rewrite <- H1. rewrite H0. easy.
-         rewrite H0.        
-
-         simpl in H1.
-         rewrite <- H1. simpl. apply f_equal.
-         
-         now rewrite extract_interp_zero.
-         
-         case_eq (N.to_nat (n0 + i)); intros; rewrite H3 in H1.
-         rewrite H0.
-         rewrite <- H1. easy.
-         
-         rewrite H0.
-         now rewrite extract_interp_all.
-         
-         rewrite H1 in H. now contradict H.
-Qed.
-
-  Lemma Npos_dist: forall p p0: positive, (Npos (p + p0))%N = (Npos p + Npos p0)%N.
-  Proof. intros. case p in *; case p0 in *; easy. Qed.
-
-  Lemma not_ltb2: forall (n0 n1 i: N), (n1 >= n0 + i)%N -> (n1 <? n0 + i)%N = false.
-  Proof. intro n0.
-         induction n0.
-         intros. simpl in *.
-         now apply N.ltb_nlt in H.
-
-         intros. simpl.
-         case_eq i.
-         intros. subst. simpl in H.
-         now apply N.ltb_nlt in H.
-         intros. subst.
-         apply N.ltb_nlt in H.
-         now rewrite Npos_dist.
-  Qed.
-
-Lemma valid_check_bbExtract pos lres : C.valid rho (check_bbExtract pos lres).
-Proof.
-      unfold check_bbExtract.
-      case_eq (S.get s pos); [intros _|intros l1 [ |l] Heq1]; try now apply C.interp_true.
-      case_eq (Lit.is_pos l1); intro Heq2; simpl; try now apply C.interp_true.
-      case_eq (Lit.is_pos lres); intro Heq3; simpl; try now apply C.interp_true.
-      case_eq (t_form .[ Lit.blit l1]); try (intros; now apply C.interp_true). intros a1 bs1 Heq4.
-      case_eq (t_form .[ Lit.blit lres]); try (intros; now apply C.interp_true).
-      intros a bsres Heq5.
-      case_eq (t_atom .[ a]); try (intros; now apply C.interp_true).
-      intros [ | | | | | | | | | | ]  a1'  Heq6; try (intros; now apply C.interp_true).
-      (* BVextract *)
-    - case_eq ((a1 == a1')); simpl; intros Heq7; try (now apply C.interp_true).
-        case_eq (
-          check_extract bs1 bsres i (n0 + i) &&
-          (N.of_nat (Datatypes.length bs1) =? n1)%N && (n0 + i <=? n1)%N
-        ); simpl; intros Heq8; try (now apply C.interp_true).
-
-        unfold C.valid. simpl. rewrite orb_false_r.
-        unfold Lit.interp. rewrite Heq3.
-        unfold Var.interp.
-        rewrite wf_interp_form; trivial. rewrite Heq5. simpl.
-
-        apply BITVECTOR_LIST.bv_eq_reflect.
-
-        generalize wt_t_atom. unfold Atom.wt. unfold is_true.
-        rewrite PArray.forallbi_spec;intros.
-
-        pose proof (H a). 
-        assert (a < PArray.length t_atom).
-        { apply PArray.get_not_default_lt. rewrite def_t_atom. rewrite Heq6. easy. }
-        specialize (@H0 H1). rewrite Heq6 in H0. simpl in H0.
-        rewrite !andb_true_iff in H0. destruct H0.
-
-        unfold get_type' in H0. unfold v_type in H0.
-        case_eq (t_interp .[ a]).
-        intros v_typea v_vala Htia. rewrite Htia in H0.
-        case_eq (v_typea);  intros; rewrite H3 in H0; try (now contradict H2).
-        rename H0 into Hv.
-
-        generalize (Hs pos). intros HSp. unfold C.valid in HSp. rewrite Heq1 in HSp.
-        unfold C.interp in HSp. unfold existsb in HSp. rewrite orb_false_r in HSp.
-        unfold Lit.interp in HSp. rewrite Heq2 in HSp. unfold Var.interp in HSp.
-        rewrite rho_interp in HSp. rewrite Heq4 in HSp. simpl in HSp.
-
-        apply BITVECTOR_LIST.bv_eq_reflect in HSp.
-
-        unfold get_type' in H2. unfold v_type in H2.
-        case_eq (t_interp .[ a1']).
-          intros v_typea1 v_vala1 Htia1. rewrite Htia1 in H2.
-        rewrite Atom.t_interp_wf in Htia1; trivial.
-        unfold apply_binop.
-        apply Typ.eqb_spec in H2.
-
-        (** case a1 = a1' **)
-        rewrite eqb_spec in Heq7; rewrite Heq7 in *.
-
-        (* interp_form_hatom_bv a = 
-                interp_bv t_i (interp_atom (t_atom .[a])) *)
-        assert (interp_form_hatom_bv a = 
-                interp_bv t_i (interp_atom (t_atom .[a]))).
-        {
-          rewrite !Atom.t_interp_wf in Htia; trivial.
-          rewrite Htia.
-          unfold Atom.interp_form_hatom_bv.
-          unfold Atom.interp_hatom.
-          rewrite !Atom.t_interp_wf; trivial.
-          rewrite Htia. easy.
-        }
-
-        rewrite H0. rewrite Heq6. simpl.
-        unfold interp_bv. unfold apply_unop.
-
-        rewrite !Atom.t_interp_wf; trivial.
-
-        revert v_vala1 Htia1. rewrite H2.
-        intros v_vala1 Htia1.
-        rewrite Htia1.
-        rewrite !Typ.cast_refl.
-        unfold Bval.
-
-        assert (H100: (N.of_nat (Datatypes.length (map (Lit.interp rho) bsres))) = n0%N).
-        {
-           rewrite !andb_true_iff in Heq8.
-           destruct Heq8 as ((Heq8a, Heq8b), Heq8c).
-           rewrite map_length.
-           specialize (@extract_interp_main bs1 bsres i n0 Heq8a).
-           intros.
-           unfold RAWBITVECTOR_LIST.bv_extr in H4.
-           assert (length (RAWBITVECTOR_LIST.extract (map (Lit.interp rho) bs1) (N.to_nat i)
-           (N.to_nat (n0 + i))) = length (map (Lit.interp rho) bsres)).
-           rewrite N.eqb_eq in Heq8b.
-           rewrite Heq8b in H4.
-           case_eq ((n1 <? n0 + i)%N); intros.
-           apply N.leb_le in Heq8c.
-           assert ((n0 + i <= n1)%N -> (n1 >= n0 + i)%N).
-           { lia. } apply H6 in Heq8c.
-           apply not_ltb2 in Heq8c. 
-           rewrite Heq8c in H5. now contradict H5.
-           rewrite H5 in H4.
-           now rewrite H4.
-           rewrite RAWBITVECTOR_LIST.length_extract, !map_length in H5.
-           assert ((n0 + i - i)%N = n0).
-           { lia. } rewrite H6 in H5.
-           now rewrite <- H5, N2Nat.id.
-           
-           rewrite map_length. 
-           rewrite N.eqb_eq in Heq8b.
-           rewrite Heq8b. unfold is_true.
-           apply N.leb_le in Heq8c.
-           assert ((n0 + i <= n1)%N -> (n1 >= n0 + i)%N).
-           { lia. } now apply H6 in Heq8c.
-           lia.
-         }
-
-        unfold BITVECTOR_LIST.of_bits, RAWBITVECTOR_LIST.of_bits.
-
-        generalize ( BITVECTOR_LIST.of_bits_size (map (Lit.interp rho) bsres)).
-
-        rewrite H100.
-        rewrite Typ.cast_refl. intros.
-        simpl.
-
-        (* interp_form_hatom_bv a1' = 
-                interp_bv t_i (interp_atom (t_atom .[a1'])) *)
-        assert (interp_form_hatom_bv a1' = 
-                interp_bv t_i (interp_atom (t_atom .[a1']))).
-        {
-          rewrite !Atom.t_interp_wf in Htia; trivial.
-          rewrite Htia1.
-          unfold Atom.interp_form_hatom_bv.
-          unfold Atom.interp_hatom.
-          rewrite !Atom.t_interp_wf; trivial.
-          rewrite Htia1. easy.
-        }
-
-        rewrite H4 in HSp.
-        unfold interp_bv in HSp.
-        rewrite Htia1 in HSp.
-        unfold interp_bv in HSp. 
-
-        revert HSp.
-
-        assert (H101: (N.of_nat (Datatypes.length (map (Lit.interp rho) bs1))) = n1).
-        {  rewrite !andb_true_iff in Heq8.
-           destruct Heq8 as ((Heq8a, Heq8b), Heq8c).
-           rewrite map_length.
-           now rewrite N.eqb_eq in Heq8b.
-        }
-
-        unfold BITVECTOR_LIST.of_bits, RAWBITVECTOR_LIST.of_bits.
-
-        generalize ( BITVECTOR_LIST.of_bits_size (map (Lit.interp rho) bs1)).
-
-        rewrite H101.
-        rewrite Typ.cast_refl. intros.
-        simpl.
-
-        rewrite HSp. simpl.
-        unfold BITVECTOR_LIST.bv_extr.
-        apply eq_rec. simpl.
-        rewrite !andb_true_iff in Heq8.
-        destruct Heq8 as (Heq8a, Heq8b).
-        specialize (@extract_interp_main bs1 bsres i n0).
-        intros.
-        rewrite map_length in H101.
-        rewrite H101 in H5. now apply H5.
-Qed.
-
-
-
-
-
-Lemma sextend_interp_zero: forall a, RAWBITVECTOR_LIST.sextend (map (Lit.interp rho) a) O =
-(map (Lit.interp rho) (sextend_lit a 0)).
-Proof. intros.
-       unfold RAWBITVECTOR_LIST.sextend.
-       case_eq a; intros; now simpl.
-Qed.
-
-Lemma sextend_interp_empty: forall i, RAWBITVECTOR_LIST.sextend (map (Lit.interp rho) []) i =
-map (Lit.interp rho) (sextend_lit [] i).
-Proof. simpl. intro i.
-       induction i.
-       - intros. now simpl.
-       - intros. simpl.
-         unfold RAWBITVECTOR_LIST.sextend in *.
-         simpl. rewrite IHi.
-         assert (Lit.interp rho Lit._false = false).
-           { specialize (Lit.interp_false rho wf_rho). intros.
-              rewrite <- not_true_iff_false.
-              unfold not in *.
-              intros. now apply H. }
-        now rewrite H.
- Qed.
-
-Lemma sextend_interp_all: forall a i, RAWBITVECTOR_LIST.sextend (map (Lit.interp rho) a) i =
-map (Lit.interp rho) (sextend_lit a i).
-Proof. intro a.
-       induction a as [ | xa xsa IHa].
-       - intros. simpl.
-         induction i.
-         + intros. now simpl.
-         + intros. unfold RAWBITVECTOR_LIST.sextend in *.
-           simpl. rewrite IHi.
-           assert (Lit.interp rho Lit._false = false).
-           { specialize (Lit.interp_false rho wf_rho). intros.
-              rewrite <- not_true_iff_false.
-              unfold not in *.
-              intros. now apply H. }
-           now rewrite H.
-        - intros. 
-          induction i.
-          + now simpl.
-          + unfold RAWBITVECTOR_LIST.sextend, zextend_lit in *.
-            simpl in *. rewrite <- IHi.
-           assert (Lit.interp rho Lit._false = false).
-           { specialize (Lit.interp_false rho wf_rho). intros.
-              rewrite <- not_true_iff_false.
-              unfold not in *.
-              intros. now apply H. }
-           reflexivity.
-Qed.
 
 Lemma sextend_interp_main: forall bs1 bsres (n i: N),
                            check_sextend bs1 bsres i = true ->
